chore: hide `null`-related things, document API, update tests, fix `meta` becoming a keyword

cvc5.lean
@@ -15,60 +15,330 @@ import cvc5.Types
 
 
 
-/-! # Cvc5 low-level API -/
+/-! # Cvc5 Lean 4 API
+
+This library exposes the `C++` API of the [cvc5] SMT solver in Lean 4. While this library tries to
+stay as close as possible to the `C++` API, some changes are required to preserve Lean 4's soundness
+and memory/thread safety.
+
+[cvc5]: https://cvc5.github.io (cvc5 official github.io page)
+
+The main issue is dealing with the fact that for some types, the values created by cvc5 are only
+safe to use as long the *"manager"* that created them is alive in memory. This is the case for
+terms, sorts, solvers, *etc.* Also, none of these types are thread-safe, because their manager
+isn't.
+
+This library blocks unsafe usage of these types through a pattern resembling Lean's `ST.Ref` type.
+In practice, this means most functions in this library make use of the `cvc5.Env` monadic
+environment.
+
+Most important sections of this documentation:
+
+- `Env`ironment monad and `Solver` (scoped) type definitions
+- [Basic scoped types](#Main-scoped-types), *e.g.* terms (`Term`) and sorts (`Srt`)
+- [`Srt`](#Srt-interface) and [`Term`](#Term-interface) interfaces
+- [`Solver` interface](#Solver-interface)
+-/
 namespace cvc5
 
 
 
-/-! ## Basic types -/
+/-! ## Cvc5 monadic environment -/
 
 
 
-/-- Error type. -/
-inductive Error where
-  | missingValue
-  | error (msg : String)
-  | recoverable (msg : String)
-  | unsupported (msg : String)
-  | option (msg : String)
-  | parsing (msg : String)
-deriving Repr
+/-- `TermManager` underlying opaque type. -/
+private opaque TermManagerImpl : NonemptyType.{0}
 
-namespace Error
+/-- Manager for cvc5 terms. -/
+private def TermManager : Type := TermManagerImpl.type
 
-def toIO : Error → IO.Error
-  | .missingValue => IO.Error.userError "missing value"
-  | .error msg => IO.Error.userError s!"{msg}"
-  | .recoverable msg => IO.Error.userError s!"[recoverable] {msg}"
-  | .unsupported msg => IO.Error.userError s!"[unsupported] {msg}"
-  | .option msg => IO.Error.userError s!"[option] {msg}"
-  | .parsing msg => IO.Error.userError s!"[parsing] {msg}"
+namespace TermManager
 
-/-- String representation of an error. -/
-protected def toString : Error → String :=
-  toString ∘ repr
+private instance : Nonempty TermManager := TermManagerImpl.property
 
-/-- Panics on errors, otherwise yields the `ok` result. -/
-def unwrap! [Inhabited α] : Except Error α → α
-| .ok a => a
-| .error e => panic! e.toString
+/-- Constructor. -/
+@[extern "termManager_new"]
+private opaque new : Unit → BaseIO TermManager
 
-instance : ToString Error :=
-  ⟨Error.toString⟩
+end TermManager
 
-end Error
 
-section variable [Monad m] [MonadExcept Error m] (msg : String)
 
-def throwMissingValue : m α := throw <| Error.missingValue
+/-- Environment monad for most `cvc5` functions, based on Lean's `ST.Ref`.
 
-protected def throw : m α := throw <| Error.error msg
-def throwRecoverable : m α := throw <| Error.recoverable msg
-def throwUnsupported : m α := throw <| Error.unsupported msg
-def throwOption : m α := throw <| Error.option msg
-def throwParsing : m α := throw <| Error.parsing msg
+`Env ω α` represents code producing a value of type `α` in *scope* `ω`. In `C++`-level terms, the
+"scope" corresponds to a specific *term manager* being alive, which means everything created by this
+manager is legal to use: terms, sorts, solvers, *etc.*
+
+As a consequence most types in this library take a scope type parameter `ω` that encode scope
+traceability as type-checking, similar to Rust's lifetimes. See for instance `Term ω` and `Solver ω`
+which can only be created inside an `Env ω` environment.
+
+For technical details on how this scoping works, see `cvc5.run`.
+-/
+structure Env (ω : Type) (α : Type) where
+/-- Private constructor from a term manager reader. -/
+private ofRaw ::
+  /-- Private accessor to the term manager reader. -/
+  private toRaw : ReaderT cvc5.TermManager (ExceptT Error BaseIO) α
+
+/-- Runs `Env ω` code, also available as `cvc5.Env.run`.
+
+# Scoping with `ω`
+
+Notice the type of the `code` argument is `{ω : Type} → Env ω α`, **not** `Env ω α` with `ω` a
+type parameter of the `run` function. This means that whatever `ω` will end up being passed to
+`code`, *it cannot escape its scope* which is the body of this `run` function.
+
+For instance, consider a hypothetical function `producesTerm : {ω : Type} → Env ω (Term ω)`.
+Remember `Term ω` is the type of terms that are only legal for scope `ω`, *i.e.* inside an `Env ω`.
+If we tried to `run` this function then the `α` in `run`'s signature would need to be `Term ω`, but
+this is impossible as `ω` cannot exist outside the `run` function.
+-/
+protected def run (code : {ω : Type} → Env ω α) : ExceptT Error BaseIO α := do
+  let tm ← TermManager.new ()
+  (@code Unit).toRaw tm
+
+/-- Convenience wrapper around `cvc5.run`/`Env.run` to run `Env ω` code in `IO`.
+
+Also available as `cvc5.Env.runIO`.
+-/
+protected def runIO (code : {ω : Type} → Env ω α) : IO α := fun world =>
+  match cvc5.run code world with
+  | .ok (.ok res) world => .ok res world
+  | .ok (.error err) world => .error err.toIO world
+
+namespace Env
+
+export cvc5 (run runIO)
+
+instance : Monad (Env ω) where
+  pure := (⟨pure ·⟩)
+  bind | ⟨code⟩, f => ⟨fun tm => code tm >>= (f · |>.toRaw tm)⟩
+
+instance : MonadExcept Error (Env ω) where
+  throw e := ⟨fun _ => throw e⟩
+  tryCatch | ⟨code⟩, errorDo => ofRaw fun tm world =>
+    match code tm world with
+    | okay@(.ok (.ok _) _) => okay
+    | error@(.error _ _) => error
+    | .ok (.error e) world => errorDo e |>.toRaw tm world
+
+instance : MonadLift (ST IO.RealWorld) (Env ω) where
+  monadLift stCode := ofRaw fun _ => stCode
+
+instance : MonadLift (Except Error) (Env ω) where
+  monadLift excCode := ofRaw fun _ => excCode
+
+instance : MonadLift IO (Env ω) where
+  monadLift ioCode := ofRaw fun _ => do
+    match ← ioCode.toBaseIO with
+    | .ok res => return res
+    | .error e => throw <| Error.error s!"[IO] {e}"
+
+-- sanity
+example : MonadLiftT BaseIO (Env ω) := inferInstance
+
+/-- Runs `TermManager`-taking `Env ω` code. -/
+private def managerDoM (f : TermManager → Env ω α) : Env ω α :=
+  ofRaw fun tm => (f tm |>.toRaw tm)
+
+/-- Runs `TermManager`-taking `Except Error` code. -/
+private def managerDo? (f : TermManager → Except Error α) : Env ω α :=
+  managerDoM (liftM ∘ f)
+
+/-- Runs a `TermManager`-taking function. -/
+private def managerDo (f : TermManager → α) : Env ω α :=
+  managerDoM (pure ∘ f)
+
+
+
+-- helpers for C++ to produce `Env ω _` values
+section ffi_helpers
+
+@[export ffi_env_pure]
+private def ffi_env_pure (a : α) : Env ω α :=
+  pure a
+
+@[export ffi_env_throw]
+private def ffi_env_throw (cppError : String) : Env ω α :=
+  throw <| .error s!"[ffi] {cppError}"
+
+end ffi_helpers
+
+end Env
+
+
+
+/-! ## `Solver` -/
+
+
+
+namespace Solver
+
+/-- `Solver.Raw` underlying opaque type, compiles to the `C++` version. -/
+private opaque RawImpl : NonemptyType.{0}
+
+/-- A `C++` cvc5 solver. -/
+private def Raw : Type := RawImpl.type
+
+
+
+private opaque InputParserImpl : NonemptyType.{0}
+
+/-- Solver input parser -/
+private def InputParser : Type := InputParserImpl.type
+
+end Solver
+
+/-- A solver under an `ω`-scope.
+
+> See `Env`'s documentation for details regarding `ω`-scoping.
+-/
+structure Solver (ω : Type) where
+/-- Private constructor. -/
+private mk' ::
+  /-- Private accessor to the underlying unsafe solver. -/
+  private toRaw : Solver.Raw
+  /-- Private accessor for the solver's (mutable reference to) its input parser.
+
+  The input parser of a solver is created lazily when first asked to parse commands; see
+  `Solver.parseSmtLib` for instance.
+  -/
+  private parser? : IO.Ref (Option Solver.InputParser)
+
+
+
+/-! ## Main scoped types -/
+
+
+
+/-- `Srt` underlying opaque type, compiles to the `C++` version. -/
+private opaque Srt.Impl : NonemptyType.{0}
+/-- The sort of a cvc5 term. -/
+@[irreducible]
+def Srt : (ω : Type) → Type := fun _ => Srt.Impl.type
+
+/-- `Op` underlying opaque type, compiles to the `C++` version. -/
+private opaque Op.Impl : NonemptyType.{0}
+/-- A cvc5 term. -/
+@[irreducible]
+def Op : (ω : Type) → Type := fun _ => Op.Impl.type
+
+/-- `Term` underlying opaque type, compiles to the `C++` version. -/
+private opaque Term.Impl : NonemptyType.{0}
+/-- A cvc5 term. -/
+@[irreducible]
+def Term : (ω : Type) → Type := fun _ => Term.Impl.type
+
+
+
+/-- `Proof` underlying opaque type, compiles to the `C++` version. -/
+private opaque Proof.Impl : NonemptyType.{0}
+
+/-- A cvc5 proof.
+
+Proofs are trees and every proof object corresponds to the root step of a proof. The branches of the
+root step are the premises of the step.
+-/
+@[irreducible]
+def Proof : (ω : Type) → Type := fun _ => Proof.Impl.type
+
+
+
+/-- `Result` underlying opaque type, compiles to the `C++` version. -/
+private opaque Result.Impl : NonemptyType.{0}
+
+/-- Encapsulation of a three-valued solver result, with explanations. -/
+@[irreducible]
+def Result : Type := Result.Impl.type
+
+
+
+
+
+namespace Solver
+
+-- ## Helpers over raw (`C++`) solvers
+namespace Raw
+
+private instance : Nonempty Raw := RawImpl.property
+
+/-- Constructor.
+
+Constructs solver instance from a given term manager instance.
+
+- `tm`: The associated term manager.
+-/
+@[extern "solver_new"]
+private opaque new : TermManager → Solver.Raw
+
+end Raw
+
+-- ## Helpers over a solver's input parser
+namespace InputParser
+
+instance : Nonempty InputParser := InputParserImpl.property
+
+/-- Private constructor. -/
+@[extern "inputParser_new"]
+private opaque new : Solver.Raw → InputParser
+
+/-- Parses some SMT-LIB commands. -/
+@[extern "inputParser_parseCommands"]
+private opaque parseCommands :
+  (raw : Solver.Raw) → (inputParser : InputParser) → (query : String) → Except Error String
+
+end InputParser
+
+/-- Private constructor from a term manager. -/
+private def ofManager (tm : TermManager) : BaseIO (Solver ω) := do
+  let parser? ← IO.mkRef none
+  return {toRaw := Raw.new tm, parser?}
+
+/-- Creates an `ω`-scoped solver inside an `Env ω`. -/
+def new : Env ω (Solver ω) := Env.managerDoM (liftM ∘ ofManager)
+
+section variable (solver : Solver ω)
+
+/-- Runs `Solver.Raw`-taking `Env ω` code. -/
+private def rawSolverDo (f : Solver.Raw → Env ω α) : Env ω α :=
+  f solver.toRaw
+
+/-- Runs `Solver.Raw`-taking `Except Error` code. -/
+private def rawSolverDo? (f : Solver.Raw → Except Error α) : Env ω α :=
+  solver.rawSolverDo (liftM ∘ f)
+
+/-- The solver's internal `InputParser`.
+
+If the solver has no input parser, a new one is created and stored as the `Solver`'s `parser?`.
+-/
+private def inputParser : Env ω InputParser := do
+  if let some parser ← solver.parser?.get then
+    return parser
+  else
+    let parser := InputParser.new solver.toRaw
+    solver.parser?.set parser
+    return parser
 
 end
+
+
+
+-- helpers for C++ to work with `Solver ω` values
+section ffi_helpers
+
+@[export ffi_solver_to_raw]
+private def ffi_solver_to_raw : Solver ω → Solver.Raw := toRaw
+
+end ffi_helpers
+
+end Solver
+
+
+
+/-! ## Helpers over basic types -/
 
 
 namespace Kind
@@ -279,56 +549,9 @@ instance : Hashable InputLanguage := ⟨InputLanguage.hash⟩
 
 end InputLanguage
 
-private opaque ResultImpl : NonemptyType.{0}
-
-/-- Encapsulation of a three-valued solver result, with explanations. -/
-def Result : Type := ResultImpl.type
-
-namespace Result
-
-instance : Nonempty Result := ResultImpl.property
-
-/-- Comparison for structural equality. -/
-protected extern_def beq : Result → Result → Bool
-
-instance : BEq Result := ⟨Result.beq⟩
-
-/-- Hash function for cvc5 sorts. -/
-protected extern_def hash : Result → UInt64
-
-instance : Hashable Result := ⟨Result.hash⟩
-
-/-- True if this result is from a satisfiable `checkSat` or `checkSatAssuming` query. -/
-extern_def isSat : Result → Bool
-
-/-- True if this result is from a unsatisfiable `checkSat` or `checkSatAssuming` query. -/
-extern_def isUnsat : Result → Bool
-
-/-- True if this result is from a `checkSat` or `checkSatAssuming` query and cvc5 was not able to
-determine (un)satisfiability.
--/
-extern_def isUnknown : Result → Bool
-
-/-- An explanation for an unknown query result.
-
-Note that if the result is (un)sat, this function returns `UnknownExplanation.UNKNOWN_REASON`.
--/
-extern_def getUnknownExplanation : Result → UnknownExplanation
-with
-  /-- An explanation for an unknown query result, `none` if the result in not unknown. -/
-  getUnknownExplanation? (res : Result) : Option UnknownExplanation :=
-    if ¬ res.isUnknown then none else res.getUnknownExplanation
-
-/-- A string representation of this result. -/
-protected extern_def toString : Result → String
-
-instance : ToString Result := ⟨Result.toString⟩
-
-end Result
 
 
-
-/-! ## FFI constructor
+/- ## FFI constructor
 
 The following constructors are only used by C++ to inject values as `Except Error _`.
 -/
@@ -363,271 +586,255 @@ end ffi_except_constructors
 
 
 
-/-! ## Environment, private `TermManager`, and `Solver`-related definitions -/
-
-
-
-private opaque TermManagerImpl : NonemptyType.{0}
-
-/-- Manager for cvc5 terms. -/
-private def TermManager : Type := TermManagerImpl.type
-
-namespace TermManager
-
-instance : Nonempty TermManager := TermManagerImpl.property
-
-@[extern "termManager_new"]
-private opaque new : Unit → BaseIO TermManager
-
-end TermManager
-
-
-structure Env (ω : Type) (α : Type) where
-private ofRaw ::
-  toRaw : ReaderT cvc5.TermManager (ExceptT Error BaseIO) α
-
-protected def run (code : {ω : Type} → Env ω α) : ExceptT Error BaseIO α := do
-  let tm ← TermManager.new ()
-  (@code Unit).toRaw tm
-
-protected def runIO (code : {ω : Type} → Env ω α) : IO α := fun world =>
-  match cvc5.run code world with
-  | .ok (.ok res) world => .ok res world
-  | .ok (.error err) world => .error err.toIO world
-
-namespace Env
-
-instance : Monad (Env ω) where
-  pure := (⟨pure ·⟩)
-  bind | ⟨code⟩, f => ⟨fun tm => code tm >>= (f · |>.toRaw tm)⟩
-
-instance : MonadExcept Error (Env ω) where
-  throw e := ⟨fun _ => throw e⟩
-  tryCatch | ⟨code⟩, errorDo => ofRaw fun tm world =>
-    match code tm world with
-    | okay@(.ok (.ok _) _) => okay
-    | error@(.error _ _) => error
-    | .ok (.error e) world => errorDo e |>.toRaw tm world
-
-instance : MonadLift (ST IO.RealWorld) (Env ω) where
-  monadLift stCode := ofRaw fun _ => stCode
-
-instance : MonadLift (Except Error) (Env ω) where
-  monadLift excCode := ofRaw fun _ => excCode
-
-instance : MonadLift IO (Env ω) where
-  monadLift ioCode := ofRaw fun _ => do
-    match ← ioCode.toBaseIO with
-    | .ok res => return res
-    | .error e => throw <| Error.error s!"[IO] {e}"
-
--- sanity
-example : MonadLiftT BaseIO (Env ω) := inferInstance
-
-private def managerDoM (f : TermManager → Env ω α) : Env ω α :=
-  ofRaw fun tm => (f tm |>.toRaw tm)
-
-private def managerDo? (f : TermManager → Except Error α) : Env ω α :=
-  managerDoM (liftM ∘ f)
-
-private def managerDo (f : TermManager → α) : Env ω α :=
-  managerDoM (pure ∘ f)
-
-
-
-/-!
-helpers for C++ to produce `Env ω _` values.
--/
-
-@[export ffi_env_pure]
-private def ffi_env_pure (a : α) : Env ω α :=
-  pure a
-
-@[export ffi_env_pure_string]
-private def ffi_env_pure_string (a : String) : Env ω String :=
-  pure a
-
-@[export ffi_env_throw]
-private def ffi_env_throw (cppError : String) : Env ω α :=
-  throw <| .error s!"[ffi] {cppError}"
-
-end Env
-
-
-
-namespace Solver
-
-private opaque RawImpl : NonemptyType.{0}
-
-/-- A cvc5 solver. -/
-private def Raw : Type := RawImpl.type
-
-namespace Raw
-
-instance : Nonempty Raw := RawImpl.property
-
-/-- Constructor.
-
-Constructs solver instance from a given term manager instance.
-
-- `tm`: The associated term manager.
--/
-@[extern "solver_new"]
-private opaque new : TermManager → Solver.Raw
-
-end Raw
-
-
-/-! ### Solver input parser -/
-
-private opaque InputParserImpl : NonemptyType.{0}
-
-/-- Solver input parser -/
-private def InputParser : Type := InputParserImpl.type
-
-namespace InputParser
-
-instance : Nonempty InputParser := InputParserImpl.property
-
-@[extern "inputParser_new"]
-private opaque new : Solver.Raw → InputParser
-
-@[extern "inputParser_parseCommands"]
-private opaque parseCommands :
-  (raw : Solver.Raw) → (inputParser : InputParser) → (query : String) → Except Error String
-
-end InputParser
-
-end Solver
-
-structure Solver (ω : Type) where
-private mk' ::
-  /-- Underlying raw solver. -/
-  private toRaw : Solver.Raw
-  /-- Parser placeholder. -/
-  private parser? : IO.Ref (Option Solver.InputParser)
-
-namespace Solver
-
-private def ofManager (tm : TermManager) : BaseIO (Solver ω) := do
-  let parser? ← IO.mkRef none
-  return {toRaw := Raw.new tm, parser?}
-
-def new : Env ω (Solver ω) := Env.managerDoM (liftM ∘ ofManager)
-
-section variable (solver : Solver ω)
-
-private def rawSolverDo (f : Solver.Raw → Env ω α) : Env ω α :=
-  f solver.toRaw
-
-private def rawSolverDo? (f : Solver.Raw → Except Error α) : Env ω α :=
-  solver.rawSolverDo (liftM ∘ f)
-
-private def inputParserDoM (f : InputParser → Env ω α) : Env ω α := do
-  if let some parser ← solver.parser?.get then f parser else
-    let parser := InputParser.new solver.toRaw
-    solver.parser?.set parser
-    f parser
-
-private def inputParser : Env ω InputParser := do
-  if let some parser ← solver.parser?.get then
-    return parser
-  else
-    let parser := InputParser.new solver.toRaw
-    solver.parser?.set parser
-    return parser
-
-/-- Parses some SMT-LIB commands and returns the output.
-
-- `commands` The SMT-LIB commands to parse.
-- `catchErrors` If true, this function fails if the parser's output contains errors. Otherwise does
-  not look at the output and simply returns it.
--/
-def parseSmtLibWithOutput (commands : String) (catchErrors : Bool := true) : Env ω String := do
-  let parser ← solver.inputParser
-  let output ← parser.parseCommands solver.toRaw commands
-  if catchErrors then
-    let output := output.trim
-    if let some err := output.splitOn "\n" |> findError? then
-      cvc5.throwParsing s!"{err}\n\n```output\n{output}\n```"
-  return output
-where
-  findError? : List String → Option String
-    | line :: tail =>
-      if line.trimLeft.startsWith "(error"
-      then extractError none 0 (line :: tail)
-      else findError? tail
-    | [] => none
-  extractError (err? : Option String) (paren : Int) : List String → String
-    | line :: tail =>
-      let paren := parenBalance line paren
-      let err := err?.map (s!"{·}\n{line}") |>.getD line
-      if paren = 0 then attemptErrorCleanup err
-      else extractError err paren tail
-    | [] => err? |>.getD "cannot extract parsing error: reached EOI"
-  parenBalance (s : String) (current : Int) : Int := Id.run do
-    let mut balance := current
-    for i in [0:s.length] do
-      match s.get ⟨i⟩ with
-      | '(' => balance := balance + 1
-      | ')' => balance := balance - 1
-      | _ => pure ()
-    return balance
-  attemptErrorCleanup (s : String) :=
-    let (pref, suff) := ("(error \"", "\")")
-    if s.startsWith pref ∧ s.endsWith suff
-    then s.drop pref.length |>.dropRight suff.length
-    else s
-
-/-- Parses some SMT-LIB commands.
-
-Fails if an error is detected in the parser's output.
--/
-def parseSmtLib (commands : String) : Env ω Unit := do
-  let _output ← solver.parseSmtLibWithOutput commands (catchErrors := true)
-
-end
-
-
-
-/-!
-Helpers for C++ to work with `Solver ω` values.
--/
-
-@[export ffi_solver_to_raw]
-private def ffi_solver_to_raw : Solver ω → Solver.Raw := toRaw
-
-end Solver
-
-
-
-
-private opaque SrtImpl : NonemptyType.{0}
-
-/-- The sort of a cvc5 term. -/
-@[irreducible]
-def Srt : (ω : Type) → Type := fun _ => SrtImpl.type
+-- ## Internal definitions
+section internal
 
 namespace Srt
 
-private theorem typeDef : Srt ω = SrtImpl.type :=
+private theorem typeDef : Srt ω = Srt.Impl.type :=
   by unfold Srt ; rfl
 
-private def toImpl : (srt : Srt ω) → SrtImpl.type :=
+private def toImpl : (srt : Srt ω) → Srt.Impl.type :=
   by rw [typeDef] ; exact id
 
-private def ofImpl : (srt : SrtImpl.type) → Srt ω :=
+private def ofImpl : (srt : Srt.Impl.type) → Srt ω :=
   by rw [typeDef] ; exact id
 
-instance instNonemptySort : Nonempty (Srt ω) :=
-  by rw [typeDef] ; exact SrtImpl.property
+instance : Nonempty (Srt ω) :=
+  by rw [typeDef] ; exact Srt.Impl.property
 
 /-- The null sort. -/
-extern_def null' as "null" : Unit → Srt ω
-@[inherit_doc null']
-def null : Env ω (Srt ω) := pure <| null' ()
+private extern_def null : Unit → Srt ω
 
-private instance : Inhabited (Srt ω) := ⟨null' ()⟩
+-- should not expose this
+private instance : Inhabited (Srt ω) := ⟨null ()⟩
+
+end Srt
+
+namespace Term
+
+private theorem typeDef : Term ω = Term.Impl.type :=
+  by unfold Term ; rfl
+
+instance instNonemptyTerm : Nonempty (Term ω) :=
+  by rw [typeDef] ; exact Term.Impl.property
+
+/-- The null term. -/
+private extern_def null : Unit → Term ω
+/-- Determine if this term is nullary. -/
+private extern_def isNull : Term ω → Bool
+
+private instance : Inhabited (Term ω) := ⟨null ()⟩
+
+end Term
+
+namespace Op
+
+private theorem typeDef : Op ω = Op.Impl.type :=
+  by unfold Op ; rfl
+
+instance instNonemptyOp : Nonempty (Op ω) :=
+  by rw [typeDef] ; exact Op.Impl.property
+
+/-- The null operator. -/
+private extern_def null : Unit → Op ω
+
+/-- Determine if this operator is nullary. -/
+private extern_def isNull : Op ω → Bool
+
+private instance : Inhabited (Op ω) := ⟨null ()⟩
+
+end Op
+
+
+namespace Proof
+
+private theorem typeDef : Proof ω = Proof.Impl.type :=
+  by unfold Proof ; rfl
+
+instance : Nonempty (Proof ω) :=
+  by rw [typeDef] ; exact Proof.Impl.property
+
+/-- The null proof. -/
+extern_def null' as "null" : Unit → Proof ω
+@[inherit_doc null']
+def null : Env ω (Proof ω) := pure <| null' ()
+
+instance : Inhabited (Proof ω) := ⟨null' ()⟩
+
+end Proof
+
+namespace Result
+
+private theorem typeDef : Result = Result.Impl.type :=
+  by unfold Result ; rfl
+
+instance : Nonempty Result :=
+  by rw [typeDef] ; exact Result.Impl.property
+
+end Result
+
+end internal
+
+
+
+/-! ## `Srt` interface -/
+
+
+
+extern_env_defs [ω] in "termManager"
+
+  /-- Get the Boolean sort. -/
+  def getBooleanSort, protected Srt.Boolean : Srt ω
+
+  /-- Get the Integer sort. -/
+  def getIntegerSort, protected Srt.Integer : Srt ω
+
+  /-- Get the Real sort. -/
+  def getRealSort, protected Srt.Real : Srt ω
+
+  /-- Get the regular expression sort. -/
+  def getRegExpSort, protected Srt.RegExp : Srt ω
+
+  /-- Get the rounding mode sort. -/
+  def getRoundingModeSort, protected Srt.RoundingModeSort : Srt ω
+
+  /-- Get the string sort. -/
+  def getStringSort, protected Srt.StringSort : Srt ω
+
+  /-- Create an array sort.
+
+  - `indexSort` The array index sort.
+  - `elemSort` The array element sort.
+  -/
+  def? mkArraySort, Srt.mkArray : (indexSort elemSort : Srt ω) → Srt ω
+
+  /-- Create a bit-vector sort.
+
+  - `size` The bit-width of the bit-vector sort.
+  -/
+  def? mkBitVectorSort, Srt.mkBitVector : (size : UInt32) → Srt ω
+
+  /-- Create a floating-point sort.
+
+  - `exp` The bit-width of the exponent of the floating-point sort.
+  - `sig` The bit-width of the significand of the floating-point sort.
+  -/
+  def? mkFloatingPointSort, Srt.mkFloatingPoint : (exp sig : UInt32) → Srt ω
+
+  /-- Create a finite-field sort from a given string of base n.
+
+  - `size` The modulus of the field. Must be a prime.
+  -/
+  private def? mkFiniteFieldSortFromString :
+    (size : String) → (base : UInt32 := 10) → Srt ω
+
+@[inherit_doc mkFiniteFieldSortFromString]
+def mkFiniteFieldSort (size : Nat) : Env ω (Srt ω) :=
+  mkFiniteFieldSortFromString (toString size) 10
+
+@[inherit_doc mkFiniteFieldSort]
+abbrev Srt.mkFiniteField := @mkFiniteFieldSort
+
+@[inherit_doc mkFiniteFieldSortFromString]
+def mkFiniteFieldSort? (size : Nat) : Env ω (Option (Srt ω)) := do
+  try some <$> mkFiniteFieldSort size catch _ => return none
+
+@[inherit_doc mkFiniteFieldSort?]
+abbrev Srt.mkFiniteField? := @mkFiniteFieldSort?
+
+
+extern_env_defs [ω] in "termManager"
+
+  /-- Create function sort.
+
+  - `sorts` The sort of the function arguments.
+  - `codomain` The sort of the function return value.
+  -/
+  def? mkFunctionSort, Srt.mkFunction : (sorts : Array (Srt ω)) → (codomain : Srt ω) → Srt ω
+
+  /-- Create a predicate sort.
+
+  This is equivalent to calling `mkFunctionSort` with Boolean sort as the codomain.
+
+  - `sorts` The list of sorts of the predicate.
+  -/
+  def? mkPredicateSort, Srt.mkPredicate : (sorts : Array (Srt ω)) → Srt ω
+
+  /-- Create a tuple sort.
+
+  - `sorts` The sorts of the elements of the tuple.
+  -/
+  def? mkTupleSort, Srt.mkTuple : (sorts : Array (Srt ω)) → Srt ω
+
+  /-- Create an uninterpreted sort constructor sort.
+
+  An uninterpreted sort constructor is an uninterpreted sort with arity > 0.
+
+  - `arity` The arity of the sort (must be > 0).
+  - `symbol` The symbol of the sort.
+  -/
+  def? mkUninterpretedSortConstructorSort, Srt.mkUninterpretedSortConstructor :
+    (arity : Nat) → (symbol : String) → Srt ω
+
+  /-- Create a set parameter.
+
+  - `elemSort` The sort of the set elements.
+  -/
+  def? mkSetSort, Srt.mkSet : (sort : Srt ω) → Srt ω
+
+  /-- Create a set parameter.
+
+  - `elemSort` The sort of the set elements.
+  -/
+  def? mkBagSort, Srt.mkBag : (sort : Srt ω) → Srt ω
+
+  /-- Create a set parameter.
+
+  - `elemSort` The sort of the set elements.
+  -/
+  def? mkSequenceSort, Srt.mkSequence : (sort : Srt ω) → Srt ω
+
+  /-- Create an abstract sort. An abstract sort represents a sort for a given kind whose parameters
+  and arguments are unspecified.
+
+  The kind `k` must be the kind of a sort that can be abstracted, *i.e.* a sort that has indices or
+  arguments sorts. For example, `SortKind.ARRAY_SORT` and `SortKind.BITVECTOR_SORT` can be passed as
+  the kind `k` to this function, while `SortKind.INTEGER_SORT` and `SortKind.STRING_SORT` cannot.
+
+  **NB:** Providing the kind `SortKind.ABSTRACT_SORT` as an argument to this function returns the
+  (fully) unspecified sort, denoted `?`.
+
+  **NB:** Providing a kind `k` that has no indices and a fixed arity of argument sorts will return
+  the sort of kind `k` whose arguments are the unspecified sort. For example, `mkAbstractSort
+  SortKind.ARRAY_SORT` will return the sort `(ARRAY_SORT ? ?)` instead of the abstract sort whose
+  abstract kind is `SortKind.ARRAY_SORT`.
+  -/
+  def? mkAbstractSort, Srt.mkAbstract : (k : SortKind) → Srt ω
+
+  /-- Create an uninterpreted sort.
+
+  - `symbol` The name of the sort.
+  -/
+  def mkUninterpretedSort, Srt.mkUninterpreted : (symbol : String) → Srt ω
+
+  /-- Create a nullable sort.
+
+  - `sort` The sort of the element of the nullable.
+  -/
+  def? mkNullableSort, Srt.mkNullable : (sort : Srt ω) → Srt ω
+
+  /-- Create a sort parameter.
+
+  - `symbol` The name of the sort.
+
+  **Warning**: This function is experimental and may change in future versions.
+  -/
+  def mkParamSort, Srt.mkParam : (symbol : String) → Srt ω
+
+
+
+namespace Srt
 
 /-- A string representation of this sort. -/
 protected extern_def toString : Srt ω → String
@@ -677,292 +884,6 @@ instance : DecidableLE (Srt ω) :=
 protected extern_def hash : Srt ω → UInt64
 
 instance : Hashable (Srt ω) := ⟨Srt.hash⟩
-
-end Srt
-
-
-
-private opaque TermImpl : NonemptyType.{0}
-
-/-- A cvc5 term. -/
-@[irreducible]
-def Term : (ω : Type) → Type := fun _ => TermImpl.type
-
-namespace Term
-
-private theorem typeDef : Term ω = TermImpl.type :=
-  by unfold Term ; rfl
-
-private def toImpl : Term ω → TermImpl.type :=
-  by rw [typeDef] ; exact id
-
-private def ofImpl : TermImpl.type → Term ω :=
-  by rw [typeDef] ; exact id
-
-instance instNonemptyTerm : Nonempty (Term ω) :=
-  by rw [typeDef] ; exact TermImpl.property
-
-/-- The null term. -/
-private extern_def null' as "null" : Unit → Term ω
-@[inherit_doc null']
-def null : Env ω (Term ω) := pure <| null' ()
-
-instance : Inhabited (Term ω) := ⟨null' ()⟩
-
-/-- A string representation of this term. -/
-protected extern_def toString : Term ω → String
-
-instance : ToString (Term ω) := ⟨Term.toString⟩
-
-/-- Syntactic equality operator. -/
-protected extern_def beq : (Term ω) → (Term ω) → Bool
-
-instance : BEq (Term ω) := ⟨Term.beq⟩
-
-protected extern_def hash : (Term ω) → UInt64
-
-instance : Hashable (Term ω) := ⟨Term.hash⟩
-
-/-- Determine if this term is nullary. -/
-extern_def isNull : Term ω → Bool
-
-end Term
-
-
-
-private opaque OpImpl : NonemptyType.{0}
-
-/-- A cvc5 term. -/
-@[irreducible]
-def Op : (ω : Type) → Type := fun _ => OpImpl.type
-
-namespace Op
-
-private theorem typeDef : Op ω = OpImpl.type :=
-  by unfold Op ; rfl
-
-private def toImpl : Op ω → OpImpl.type :=
-  by rw [typeDef] ; exact id
-
-private def ofImpl : OpImpl.type → Op ω :=
-  by rw [typeDef] ; exact id
-
-instance instNonemptyOp : Nonempty (Op ω) :=
-  by rw [typeDef] ; exact OpImpl.property
-
-/-- The null operator. -/
-extern_def null' as "null" : Unit → Op ω
-@[inherit_doc null']
-def null : Env ω (Op ω) := pure <| null' ()
-
-/-- Determine if this operator is nullary. -/
-extern_def isNull : Op ω → Bool
-
-instance : Inhabited (Op ω) := ⟨null' ()⟩
-
-/-- A string representation of this term. -/
-protected extern_def toString : Op ω → String
-
-instance : ToString (Op ω) := ⟨Op.toString⟩
-
-end Op
-
-
-
-private opaque ProofImpl : NonemptyType.{0}
-
-/-- A cvc5 proof.
-
-Proofs are trees and every proof object corresponds to the root step of a proof. The branches of the
-root step are the premises of the step.
--/
-@[irreducible]
-def Proof : (ω : Type) → Type := fun _ => ProofImpl.type
-
-namespace Proof
-
-private theorem typeDef : Proof ω = ProofImpl.type :=
-  by unfold Proof ; rfl
-
-private def toImpl : Proof ω → ProofImpl.type :=
-  by rw [typeDef] ; exact id
-
-private def ofImpl : ProofImpl.type → Proof ω :=
-  by rw [typeDef] ; exact id
-
-instance instNonemptyProof : Nonempty (Proof ω) :=
-  by rw [typeDef] ; exact ProofImpl.property
-
-/-- The null proof. -/
-extern_def null' as "null" : Unit → Proof ω
-@[inherit_doc null']
-def null : Env ω (Proof ω) := pure <| null' ()
-
-instance : Inhabited (Proof ω) := ⟨null' ()⟩
-
-end Proof
-
-
-
-/-! ## User-facing definitions -/
-
-
-
-/-! ### `Srt` functions -/
-
-extern_env_defs [ω] in "termManager"
-
-  /-- Get the Boolean sort. -/
-  def getBooleanSort : Srt ω
-
-  /-- Get the Integer sort. -/
-  def getIntegerSort : Srt ω
-
-  /-- Get the Real sort. -/
-  def getRealSort : Srt ω
-
-  /-- Get the regular expression sort. -/
-  def getRegExpSort : Srt ω
-
-  /-- Get the rounding mode sort. -/
-  def getRoundingModeSort : Srt ω
-
-  /-- Get the string sort. -/
-  def getStringSort : Srt ω
-
-  /-- Create an array sort.
-
-  - `indexSort` The array index sort.
-  - `elemSort` The array element sort.
-  -/
-  def? mkArraySort : (indexSort elemSort : Srt ω) → Srt ω
-
-  /-- Create a bit-vector sort.
-
-  - `size` The bit-width of the bit-vector sort.
-  -/
-  def? mkBitVectorSort : (size : UInt32) → Srt ω
-
-  /-- Create a floating-point sort.
-
-  - `exp` The bit-width of the exponent of the floating-point sort.
-  - `sig` The bit-width of the significand of the floating-point sort.
-  -/
-  def? mkFloatingPointSort : (exp sig : UInt32) → Srt ω
-
-  /-- Create a finite-field sort from a given string of base n.
-
-  - `size` The modulus of the field. Must be a prime.
-  -/
-  private def? mkFiniteFieldSortFromString :
-    (size : String) → (base : UInt32 := 10) → Srt ω
-
-@[inherit_doc mkFiniteFieldSortFromString]
-abbrev mkFiniteFieldSort (size : Nat) : Env ω (Srt ω) :=
-  mkFiniteFieldSortFromString (toString size) 10
-@[inherit_doc mkFiniteFieldSortFromString]
-abbrev mkFiniteFieldSort? (size : Nat) : Env ω (Option (Srt ω)) := do
-  try some <$> mkFiniteFieldSort size catch _ => return none
-
-extern_env_defs [ω] in "termManager"
-
-  /-- Create function sort.
-
-  - `sorts` The sort of the function arguments.
-  - `codomain` The sort of the function return value.
-  -/
-  def? mkFunctionSort : (sorts : Array (Srt ω)) → (codomain : Srt ω) → Srt ω
-
-  /-- Create a predicate sort.
-
-  This is equivalent to calling `mkFunctionSort` with Boolean sort as the codomain.
-
-  - `sorts` The list of sorts of the predicate.
-  -/
-  def? mkPredicateSort : (sorts : Array (Srt ω)) → Srt ω
-
-  /-- Create a tuple sort.
-
-  - `sorts` The sorts of the elements of the tuple.
-  -/
-  def? mkTupleSort : (sorts : Array (Srt ω)) → Srt ω
-
-  /-- Create an uninterpreted sort constructor sort.
-
-  An uninterpreted sort constructor is an uninterpreted sort with arity > 0.
-
-  - `arity` The arity of the sort (must be > 0).
-  - `symbol` The symbol of the sort.
-  -/
-  def? mkUninterpretedSortConstructorSort : (arity : Nat) → (symbol : String) → Srt ω
-
-  /-- Create a set parameter.
-
-  - `elemSort` The sort of the set elements.
-  -/
-  def? mkSetSort : (sort : Srt ω) → Srt ω
-
-  /-- Create a set parameter.
-
-  - `elemSort` The sort of the set elements.
-  -/
-  def? mkBagSort : (sort : Srt ω) → Srt ω
-
-  /-- Create a set parameter.
-
-  - `elemSort` The sort of the set elements.
-  -/
-  def? mkSequenceSort : (sort : Srt ω) → Srt ω
-
-  /-- Create an abstract sort. An abstract sort represents a sort for a given kind whose parameters
-  and arguments are unspecified.
-
-  The kind `k` must be the kind of a sort that can be abstracted, *i.e.* a sort that has indices or
-  arguments sorts. For example, `SortKind.ARRAY_SORT` and `SortKind.BITVECTOR_SORT` can be passed as
-  the kind `k` to this function, while `SortKind.INTEGER_SORT` and `SortKind.STRING_SORT` cannot.
-
-  **NB:** Providing the kind `SortKind.ABSTRACT_SORT` as an argument to this function returns the
-  (fully) unspecified sort, denoted `?`.
-
-  **NB:** Providing a kind `k` that has no indices and a fixed arity of argument sorts will return
-  the sort of kind `k` whose arguments are the unspecified sort. For example, `mkAbstractSort
-  SortKind.ARRAY_SORT` will return the sort `(ARRAY_SORT ? ?)` instead of the abstract sort whose
-  abstract kind is `SortKind.ARRAY_SORT`.
-  -/
-  def? mkAbstractSort : (k : SortKind) → Srt ω
-
-  /-- Create an uninterpreted sort.
-
-  - `symbol` The name of the sort.
-  -/
-  def mkUninterpretedSort : (symbol : String) → Srt ω
-
-  /-- Create a nullable sort.
-
-  - `sort` The sort of the element of the nullable.
-  -/
-  def? mkNullableSort : (sort : Srt ω) → Srt ω
-
-  /-- Create a sort parameter.
-
-  - `symbol` The name of the sort.
-
-  **Warning**: This function is experimental and may change in future versions.
-  -/
-  def mkParamSort : (symbol : String) → Srt ω
-
-
-
-namespace Srt
-
-@[inherit_doc getBooleanSort]
-abbrev mkBoolean := @getBooleanSort
-
-@[inherit_doc getBooleanSort]
-abbrev mkInteger := @getIntegerSort
-
-@[inherit_doc getBooleanSort]
-abbrev mkReal := @getRealSort
 
 /-- Get the kind of this sort. -/
 extern_def getKind : Srt ω → SortKind
@@ -1162,101 +1083,33 @@ end Srt
 
 
 
-namespace Op
-
-/-- Syntactic equality operator. -/
-protected extern_def beq : Op ω → Op ω → Bool
-
-instance : BEq (Op ω) := ⟨Op.beq⟩
-
-/-- Get the kind of this operator. -/
-extern_def getKind : Op ω → Kind
-
-/-- Determine if this operator is indexed. -/
-extern_def isIndexed : Op ω → Bool
-
-/-- Get the number of indices of this operator. -/
-extern_def getNumIndices : Op ω → Nat
-
-/-- Get the index at position `i` of an indexed operator. -/
-protected extern_def get : (op : Op ω) → Fin op.getNumIndices → Term ω
-
-instance : GetElem (Op ω) Nat (Term ω) fun op i => i < op.getNumIndices where
-  getElem op i h := op.get ⟨i, h⟩
+/-! ## `Term` interface -/
 
 
-
-extern_env_defs [ω] in "termManager"
-
-  /-- Create operator of kind:
-
-  - `Kind.DIVISIBLE` (to support arbitrary precision integers)
-
-  See `cvc5.Kind` for a description of the parameters.
-
-  - `kind` The kind of the operator.
-  - `arg` The string argument to this operator.
-  -/
-  def? ofString as "mkOpOfString" : (kind : Kind) → (arg : String) → Op ω
-
-  /-- Create n-ary term of given kind from a given operator.
-
-  Create operators with `mkOp`.
-
-  - `op` The operator.
-  - `children` The children of the term.
-  -/
-  def? mkTerm as "mkTermOfOp" : (op : Op ω) → (children : Array (Term ω) := #[]) → Term ω
-
-  /-- Create operator of Kind:
-
-  - `Kind.BITVECTOR_EXTRACT`
-  - `Kind.BITVECTOR_REPEAT`
-  - `Kind.BITVECTOR_ROTATE_LEFT`
-  - `Kind.BITVECTOR_ROTATE_RIGHT`
-  - `Kind.BITVECTOR_SIGN_EXTEND`
-  - `Kind.BITVECTOR_ZERO_EXTEND`
-  - `Kind.DIVISIBLE`
-  - `Kind.FLOATINGPOINT_TO_FP_FROM_FP`
-  - `Kind.FLOATINGPOINT_TO_FP_FROM_IEEE_BV`
-  - `Kind.FLOATINGPOINT_TO_FP_FROM_REAL`
-  - `Kind.FLOATINGPOINT_TO_FP_FROM_SBV`
-  - `Kind.FLOATINGPOINT_TO_FP_FROM_UBV`
-  - `Kind.FLOATINGPOINT_TO_SBV`
-  - `Kind.FLOATINGPOINT_TO_UBV`
-  - `Kind.INT_TO_BITVECTOR`
-  - `Kind.TUPLE_PROJECT`
-
-  See `cvc5.Kind` for a description of the parameters.
-
-  - `kind` The kind of the operator.
-  - `args` The arguments (indices) of the operator.
-
-  If `args` is empty, the `Op` simply wraps the `cvc5.Kind`. The `Kind` can be used in
-  `Term.mk` directly without creating an `Op` first.
-  -/
-  def? ofIndices as "mkOpOfIndices" : (kind : Kind) → (args : Array Nat := #[]) → Op ω
-
-@[inherit_doc ofIndices]
-abbrev ofOp := @ofIndices
-
-end Op
 
 /-- Create n-ary term of given kind.
 
 - `kind` The kind of the term.
 - `children` The children of the term.
 -/
-extern_env_def? [ω] in "termManager" mkTerm :
+extern_env_def? [ω] in "termManager" mkTerm, Term.mk :
   (kind : Kind) → (children : Array (Term ω) := #[]) → Term ω
 
 namespace Term
 
-@[inherit_doc cvc5.mkTerm]
-def mk := @cvc5.mkTerm
+/-- A string representation of this term. -/
+protected extern_def toString : Term ω → String
 
-@[inherit_doc Op.mkTerm]
-def ofOp := @Op.mkTerm
+instance : ToString (Term ω) := ⟨Term.toString⟩
+
+/-- Syntactic equality operator. -/
+protected extern_def beq : (Term ω) → (Term ω) → Bool
+
+instance : BEq (Term ω) := ⟨Term.beq⟩
+
+protected extern_def hash : (Term ω) → UInt64
+
+instance : Hashable (Term ω) := ⟨Term.hash⟩
 
 extern_env_defs [ω] in "termManager"
 
@@ -1463,6 +1316,100 @@ end Term
 
 
 
+/-! ## `Op` interface -/
+
+
+
+namespace Op
+
+/-- A string representation of this term. -/
+protected extern_def toString : Op ω → String
+
+instance : ToString (Op ω) := ⟨Op.toString⟩
+
+/-- Syntactic equality operator. -/
+protected extern_def beq : Op ω → Op ω → Bool
+
+instance : BEq (Op ω) := ⟨Op.beq⟩
+
+/-- Get the kind of this operator. -/
+extern_def getKind : Op ω → Kind
+
+/-- Determine if this operator is indexed. -/
+extern_def isIndexed : Op ω → Bool
+
+/-- Get the number of indices of this operator. -/
+extern_def getNumIndices : Op ω → Nat
+
+/-- Get the index at position `i` of an indexed operator. -/
+protected extern_def get : (op : Op ω) → Fin op.getNumIndices → Term ω
+
+instance : GetElem (Op ω) Nat (Term ω) fun op i => i < op.getNumIndices where
+  getElem op i h := op.get ⟨i, h⟩
+
+extern_env_defs [ω] in "termManager"
+
+  /-- Create operator of kind:
+
+  - `Kind.DIVISIBLE` (to support arbitrary precision integers)
+
+  See `cvc5.Kind` for a description of the parameters.
+
+  - `kind` The kind of the operator.
+  - `arg` The string argument to this operator.
+  -/
+  def? ofString as "mkOpOfString" : (kind : Kind) → (arg : String) → Op ω
+
+  /-- Create n-ary term of given kind from a given operator.
+
+  Create operators with `mkOp`.
+
+  - `op` The operator.
+  - `children` The children of the term.
+  -/
+  def? mkTerm, _root_.cvc5.Term.ofOp as "mkTermOfOp" :
+    (op : Op ω) → (children : Array (Term ω) := #[]) → Term ω
+
+  /-- Create operator of Kind:
+
+  - `Kind.BITVECTOR_EXTRACT`
+  - `Kind.BITVECTOR_REPEAT`
+  - `Kind.BITVECTOR_ROTATE_LEFT`
+  - `Kind.BITVECTOR_ROTATE_RIGHT`
+  - `Kind.BITVECTOR_SIGN_EXTEND`
+  - `Kind.BITVECTOR_ZERO_EXTEND`
+  - `Kind.DIVISIBLE`
+  - `Kind.FLOATINGPOINT_TO_FP_FROM_FP`
+  - `Kind.FLOATINGPOINT_TO_FP_FROM_IEEE_BV`
+  - `Kind.FLOATINGPOINT_TO_FP_FROM_REAL`
+  - `Kind.FLOATINGPOINT_TO_FP_FROM_SBV`
+  - `Kind.FLOATINGPOINT_TO_FP_FROM_UBV`
+  - `Kind.FLOATINGPOINT_TO_SBV`
+  - `Kind.FLOATINGPOINT_TO_UBV`
+  - `Kind.INT_TO_BITVECTOR`
+  - `Kind.TUPLE_PROJECT`
+
+  See `cvc5.Kind` for a description of the parameters.
+
+  - `kind` The kind of the operator.
+  - `args` The arguments (indices) of the operator.
+
+  If `args` is empty, the `Op` simply wraps the `cvc5.Kind`. The `Kind` can be used in
+  `Term.mk` directly without creating an `Op` first.
+  -/
+  def? ofIndices as "mkOpOfIndices" : (kind : Kind) → (args : Array Nat := #[]) → Op ω
+
+@[inherit_doc ofIndices]
+abbrev ofOp := @ofIndices
+
+end Op
+
+
+
+/-! ## `Proof` interface -/
+
+
+
 namespace Proof
 
 /-- Get the proof rule used by the root step of the root. -/
@@ -1500,7 +1447,57 @@ end Proof
 
 
 
-namespace Solver variable (solver : Solver ω)
+/-! ## `Result` interface -/
+
+
+
+namespace Result
+
+/-- Comparison for structural equality. -/
+protected extern_def beq : Result → Result → Bool
+
+instance : BEq Result := ⟨Result.beq⟩
+
+/-- Hash function for cvc5 sorts. -/
+protected extern_def hash : Result → UInt64
+
+instance : Hashable Result := ⟨Result.hash⟩
+
+/-- True if this result is from a satisfiable `checkSat` or `checkSatAssuming` query. -/
+extern_def isSat : Result → Bool
+
+/-- True if this result is from a unsatisfiable `checkSat` or `checkSatAssuming` query. -/
+extern_def isUnsat : Result → Bool
+
+/-- True if this result is from a `checkSat` or `checkSatAssuming` query and cvc5 was not able to
+determine (un)satisfiability.
+-/
+extern_def isUnknown : Result → Bool
+
+/-- An explanation for an unknown query result.
+
+Note that if the result is (un)sat, this function returns `UnknownExplanation.UNKNOWN_REASON`.
+-/
+extern_def getUnknownExplanation : Result → UnknownExplanation
+with
+  /-- An explanation for an unknown query result, `none` if the result in not unknown. -/
+  getUnknownExplanation? (res : Result) : Option UnknownExplanation :=
+    if ¬ res.isUnknown then none else res.getUnknownExplanation
+
+/-- A string representation of this result. -/
+protected extern_def toString : Result → String
+
+instance : ToString Result := ⟨Result.toString⟩
+
+end Result
+
+
+
+/-! ## `Solver` interface -/
+
+
+
+namespace Solver
 
 /-- Get a string representation of the version of this solver. -/
 extern_def getVersion (solver : Solver ω) : Env ω String
@@ -1612,11 +1609,56 @@ Other aspects of printing are taken from the solver options.
 -/
 extern_def proofToString (solver : Solver ω) : (proof : Proof ω) → Env ω String
 
--- /-- Parse a string containing SMT-LIB commands.
 
--- Commands that produce a result such as `(check-sat)`, `(get-model)`, ... are executed but the
--- results are ignored.
--- -/
--- extern_def parseCommands (solver : Solver ω) : (smtLib : String) → Env ω Unit
+/-- Parses some SMT-LIB commands and returns the output.
+
+- `commands` The SMT-LIB commands to parse.
+- `catchErrors` If true, this function fails if the parser's output contains errors. Otherwise it
+  does not check the parser's output and simply returns it.
+-/
+def parseSmtLibWithOutput (solver : Solver ω)
+  (commands : String) (catchErrors : Bool := true)
+: Env ω String := do
+  let parser ← solver.inputParser
+  let output ← parser.parseCommands solver.toRaw commands
+  if catchErrors then
+    let output := output.trim
+    if let some err := output.splitOn "\n" |> findError? then
+      cvc5.throwParsing s!"{err}\n\n```output\n{output}\n```"
+  return output
+where
+  findError? : List String → Option String
+    | line :: tail =>
+      if line.trimLeft.startsWith "(error"
+      then extractError none 0 (line :: tail)
+      else findError? tail
+    | [] => none
+  extractError (err? : Option String) (paren : Int) : List String → String
+    | line :: tail =>
+      let paren := parenBalance line paren
+      let err := err?.map (s!"{·}\n{line}") |>.getD line
+      if paren = 0 then attemptErrorCleanup err
+      else extractError err paren tail
+    | [] => err? |>.getD "cannot extract parsing error: reached EOI"
+  parenBalance (s : String) (current : Int) : Int := Id.run do
+    let mut balance := current
+    for i in [0:s.length] do
+      match s.get ⟨i⟩ with
+      | '(' => balance := balance + 1
+      | ')' => balance := balance - 1
+      | _ => pure ()
+    return balance
+  attemptErrorCleanup (s : String) :=
+    let (pref, suff) := ("(error \"", "\")")
+    if s.startsWith pref ∧ s.endsWith suff
+    then s.drop pref.length |>.dropRight suff.length
+    else s
+
+/-- Parses some SMT-LIB commands.
+
+Fails if an error is detected in the parser's output.
+-/
+def parseSmtLib (solver : Solver ω) (commands : String) : Env ω Unit := do
+  let _output ← solver.parseSmtLibWithOutput commands (catchErrors := true)
 
 end Solver
