cvc5Test/Test.lean
@@ -4,22 +4,22 @@ import cvc5
 
 namespace Test
 
-open cvc5 (Solver)
+open cvc5 (Solver Srt Term)
 
-/-- info: bool = `Bool` -/
+/-- info: bool sort = `Bool` -/
 #guard_msgs in #eval cvc5.runIO do
-  let bool ← cvc5.getBooleanSort
-  println! "bool = `{bool}`"
+  let bool ← Srt.Boolean
+  println! "bool sort = `{bool}`"
 
 /-- error: not a function sort: Bool -/
 #guard_msgs in #eval cvc5.runIO do
-  let bool ← cvc5.getBooleanSort
+  let bool ← Srt.Boolean
   let _sorts ← bool.getFunctionDomainSorts
 
 /-- info: Bool.substitute [Bool → Int] = Int -/
 #guard_msgs in #eval cvc5.runIO do
-  let bool ← cvc5.getBooleanSort
-  let int ← cvc5.getIntegerSort
+  let bool ← Srt.Boolean
+  let int ← Srt.Integer
   let sub ← bool.substitute #[bool] #[int]
   println! "{bool}.substitute [{bool} → {int}] = {sub}"
 
@@ -38,13 +38,13 @@ b4 = `b4`
 conj = `(and b1 b2 b3 b4)`
 -/
 #guard_msgs in #eval cvc5.runIO do
-  let bool ← cvc5.getBooleanSort
+  let bool ← Srt.Boolean
   let solver ← Solver.new
   let b1 ← solver.declareFun "b1" #[] bool
   println! "b1 = `{b1}`"
   let b2 ← solver.declareFun "b2" #[] bool
   println! "b2 = `{b2}`"
-  let b1_and_b2 ← cvc5.Term.mk .AND #[b1, b2]
+  let b1_and_b2 ← Term.mk .AND #[b1, b2]
   println! "b1_and_b2 = `{b1_and_b2}`"
   let b3 ← solver.declareFun "b3" #[] bool
   println! "b3 = `{b3}`"
@@ -55,8 +55,8 @@ conj = `(and b1 b2 b3 b4)`
 
 /-- error: expecting a Boolean subexpression -/
 #guard_msgs in #eval cvc5.runIO do
-  let bool ← cvc5.getBooleanSort
-  let int ← cvc5.getIntegerSort
+  let bool ← Srt.Boolean
+  let int ← Srt.Integer
   let solver ← Solver.new
   let b1 ← solver.declareFun "b1" #[] bool
   let i1 ← solver.declareFun "i1" #[] int
@@ -71,8 +71,8 @@ i1_plus_zero = (+ i1 0)
 i1_plus_zero_simplified = i1
 -/
 #guard_msgs in #eval cvc5.runIO do
-  let bool ← cvc5.getBooleanSort
-  let int ← cvc5.getIntegerSort
+  let bool ← Srt.Boolean
+  let int ← Srt.Integer
   let solver ← Solver.new
 
   solver.setOption "produce-models" "true"
@@ -85,7 +85,7 @@ i1_plus_zero_simplified = i1
   println! "b1_and_b1_simplified = {b1_and_b1_simplified}"
 
   let i1 ← solver.declareFun "i1" #[] int
-  let i1_plus_zero ← i1.mkInto .ADD #[← cvc5.Term.mkInteger 0]
+  let i1_plus_zero ← i1.mkInto .ADD #[← Term.mkInteger 0]
   println! "i1_plus_zero = {i1_plus_zero}"
   let i1_plus_zero_simplified ← solver.simplify i1_plus_zero
   println! "i1_plus_zero_simplified = {i1_plus_zero_simplified}"
@@ -97,7 +97,7 @@ confirmed sat
 confirmed sat
 -/
 #guard_msgs in #eval cvc5.runIO do
-  let bool ← cvc5.getBooleanSort
+  let bool ← Srt.Boolean
   let solver ← Solver.new
   let b1 ← solver.declareFun "b1" #[] bool
   let not_b1 ← b1.mkInto .NOT
@@ -144,7 +144,7 @@ can't retrieve a symbol created by `parseCommands`
   if ¬ res.isSat then
     cvc5.throw "expected sat"
 
-  let bool ← cvc5.getBooleanSort
+  let bool ← Srt.Boolean
   let b1 ← solver.declareFun "b1" #[] bool (fresh := false)
   solver.assertFormula (← b1.mkInto .NOT)
   let res ← solver.checkSat
